try to change multi_ceval' on func to multi_ceval' on com

ASTLc_woc.v
@@ -200,20 +200,20 @@ Inductive ceval' : func_context -> com -> label -> label -> state -> state -> Pr
 
 
 (** Bridging basic ceval' to multi_ceval' *)
-Definition restk : Type := list (func * label * state).
+Definition restk : Type := list (com * label * state).
 
 Inductive middle_ceval' : func_context -> restk -> restk -> Prop :=
-  | ME_r : forall fc f l1 l2 st1 st2 stk,
-      ceval' fc (snd (fc f)) l1 l2 st1 st2 ->
-      middle_ceval' fc ((f, l1, st1) :: stk) ((f, l2, st2) :: stk)
-  | ME_re : forall fc f1 f2 l1 loc1 loc2 glb stk,
+  | ME_r : forall fc c l1 l2 st1 st2 stk,
+      ceval' fc c l1 l2 st1 st2 ->
+      middle_ceval' fc ((c, l1, st1) :: stk) ((c, l2, st2) :: stk)
+  | ME_re : forall fc c1 c2 l1 loc1 loc2 glb stk,
       single_point l1 ->
-      middle_ceval' fc ((f1, l1, (loc1, glb)) :: stk)
-        ((f2, (com_to_lable_pure (snd (fc f2))), (loc2, glb)) :: (f1, l1, (loc1, glb)) :: stk)
-  | ME_ex : forall fc f1 f2 l2 loc1 loc2 glb1 glb2 stk,
+      middle_ceval' fc ((c1, l1, (loc1, glb)) :: stk)
+        ((c2, com_to_lable_pure c2, (loc2, glb)) :: (c1, l1, (loc1, glb)) :: stk)
+  | ME_ex : forall fc c1 c2 l2 loc1 loc2 glb1 glb2 stk,
       middle_ceval' fc
-        ((f1, (com_to_lable_pure (snd (fc f1))), (loc1, glb1)) :: (f2, l2, (loc2, glb2)) :: stk)
-        ((f2, l2, (loc2, glb1)) :: stk).
+        ((c1, (com_to_lable_pure c1), (loc1, glb1)) :: (c2, l2, (loc2, glb2)) :: stk)
+        ((c2, l2, (loc2, glb1)) :: stk).
 
 Print clos_trans.
 (*
@@ -224,9 +224,9 @@ Inductive clos_trans (A : Type) (R : relation A) (x : A) : A -> Prop :=
 Definition multi_ceval' (fc : func_context) : restk -> restk -> Prop :=
   clos_trans restk (middle_ceval' fc).
 
-Lemma middle_ceval'_pure : forall fc f l1 l2 st1 st2,
-  middle_ceval' fc ((f, l1, st1) :: nil) ((f, l2, st2) :: nil) ->
-  ceval' fc (snd (fc f)) l1 l2 st1 st2.
+Lemma middle_ceval'_pure : forall fc c l1 l2 st1 st2,
+  middle_ceval' fc ((c, l1, st1) :: nil) ((c, l2, st2) :: nil) ->
+  ceval' fc c l1 l2 st1 st2.
 Proof.
   intros.
   inversion H; subst.
@@ -239,29 +239,38 @@ Qed.
 Check ceval.
 Check multi_ceval'.
 Print ceval.
-Definition ceval'_derive_multi_ceval (fc : func_context) (f : func) (st1 st2 : state) : Prop :=
-  ceval fc (snd (fc f)) st1 st2 ->
+Definition ceval'_derive_multi_ceval (fc : func_context) (c : com) (st1 st2 : state) : Prop :=
+  ceval fc c st1 st2 ->
   multi_ceval' fc
-    ((f, com_to_lable_pure (snd (fc f)), st1) :: nil)
-    ((f, com_to_lable_pure (snd (fc f)), st2) :: nil).
-
+    ((c, com_to_lable_pure c, st1) :: nil)
+    ((c, com_to_lable_pure c, st2) :: nil).
+(* 
 Definition ceval_multi_derive_ceval' (fc : func_context) (f : func) (st1 st2 : state) : Prop :=
   multi_ceval' fc
     ((f, com_to_lable_pure (snd (fc f)), st1) :: nil)
     ((f, com_to_lable_pure (snd (fc f)), st2) :: nil) ->
   ceval fc (snd (fc f)) st1 st2.
+ *)
+(* Scheme eval_abeval := Minimality for ceval Sort Prop
+  with abeval_eval := Minimality for arbitrary_eval Sort Prop. *)
 
-Scheme eval_abeval := Minimality for ceval Sort Prop
-  with abeval_eval := Minimality for arbitrary_eval Sort Prop.
-
-Check eval_abeval.
-
-Theorem ceval'_derive_multi_ceval_correct : forall fc f st1 st2,
-  ceval'_derive_multi_ceval fc f st1 st2.
+Theorem ceval'_derive_multi_ceval_correct : forall fc c st1 st2,
+  ceval'_derive_multi_ceval fc c st1 st2.
 Proof.
   unfold ceval'_derive_multi_ceval.
   intros.
-  remember (snd (fc f)) as c.
+  induction H.
+  - simpl.
+    apply t_step, ME_r.
+    apply E'_Skip.
+  - simpl.
+    apply t_step, ME_r.
+    apply E'_Ass, H.
+  - simpl.
+    apply t_step, ME_r.
+  
+  
+(*   remember (snd (fc f)) as c.
   revert f Heqc.
   induction H; intros.
   - simpl.
@@ -273,7 +282,7 @@ Proof.
     rewrite <- Heqc.
     apply E'_Ass, H.
   - simpl.
-Admitted.
+Admitted. *)
 
 Theorem ceval_multi_derive_ceval'_correct : forall fc f st1 st2,
   ceval_multi_derive_ceval' fc f st1 st2.
